02Stack/EvaluateStack.thy
@@ -7,7 +7,7 @@ inductive evaluate :: "stack_state \<Rightarrow> stack_state \<Rightarrow> bool"
 | ev_abs [simp]: "StackState (Eval (Abs t e)) s h \<leadsto>\<^sub>s StackState (Return (VAbs t e)) s h"
 | ev_app [simp]: "StackState (Eval (App e\<^sub>1 e\<^sub>2)) s h \<leadsto>\<^sub>s StackState (Eval e\<^sub>1) (SApp e\<^sub>2 # s) h" 
 | ev_let [simp]: "StackState (Eval (Let e\<^sub>1 e\<^sub>2)) s h \<leadsto>\<^sub>s 
-    StackState (Eval (subst\<^sub>e\<^sub>e 0 (Var (length\<^sub>h h)) e\<^sub>2)) s (extend\<^sub>h h e\<^sub>1)"
+    StackState (Eval (subst\<^sub>x\<^sub>e 0 (length\<^sub>h h) e\<^sub>2)) s (extend\<^sub>h h e\<^sub>1)"
 | ev_rec [simp]: "StackState (Eval (Rec vs)) s h \<leadsto>\<^sub>s StackState (Return (VRec vs)) s h" 
 | ev_proj [simp]: "StackState (Eval (Proj e l)) s h \<leadsto>\<^sub>s StackState (Eval e) (SProj l # s) h"
 | ev_inj [simp]: "StackState (Eval (Inj l ts x)) s h \<leadsto>\<^sub>s StackState (Return (VInj l ts x)) s h"
@@ -17,16 +17,16 @@ inductive evaluate :: "stack_state \<Rightarrow> stack_state \<Rightarrow> bool"
 | ev_tyabs [simp]: "StackState (Eval (TyAbs k e)) s h \<leadsto>\<^sub>s StackState (Return (VTyAbs k e)) s h" 
 | ev_tyapp [simp]: "StackState (Eval (TyApp e t)) s h \<leadsto>\<^sub>s StackState (Eval e) (STyApp t # s) h" 
 | ev_tylet [simp]: "StackState (Eval (TyLet t e)) s h \<leadsto>\<^sub>s StackState (Eval (subst\<^sub>t\<^sub>e 0 t e)) s h" 
-| ret_ref [simp]: "StackState (Return v) (SRef x # s) h \<leadsto>\<^sub>s StackState (Return v) s (update\<^sub>h h x e)"
-| ret_app [simp]: 
-    "StackState (Return (VAbs t e\<^sub>1)) (SApp e\<^sub>2 # s) h \<leadsto>\<^sub>s StackState (Eval e\<^sub>1) s (extend\<^sub>h h e\<^sub>2)"
+| ret_ref [simp]: 
+    "StackState (Return v) (SRef x # s) h \<leadsto>\<^sub>s StackState (Return v) s (update\<^sub>h h x (devalue v))"
+| ret_app [simp]: "StackState (Return (VAbs t e\<^sub>1)) (SApp e\<^sub>2 # s) h \<leadsto>\<^sub>s 
+    StackState (Eval (subst\<^sub>x\<^sub>e 0 (length\<^sub>h h) e\<^sub>1)) s (extend\<^sub>h h e\<^sub>2)"
 | ret_proj [simp]: "lookup l xs = Some x \<Longrightarrow> 
     StackState (Return (VRec xs)) (SProj l # s) h \<leadsto>\<^sub>s StackState (Eval (Var x)) s h" 
 | ret_case [simp]: "lookup l cs = Some e \<Longrightarrow> 
-    StackState (Return (VInj l ts x)) (SCase t cs # s) h \<leadsto>\<^sub>s 
-      StackState (Eval e) s (extend\<^sub>h h (Var x))"
+    StackState (Return (VInj l ts x)) (SCase t cs # s) h \<leadsto>\<^sub>s StackState (Eval (subst\<^sub>x\<^sub>e 0 x e)) s h"
 | ret_unfold [simp]: 
-    "StackState (Return (VFold t e)) (SUnfold t # s) h \<leadsto>\<^sub>s StackState (Eval (Var e)) s h" 
+    "StackState (Return (VFold t x)) (SUnfold t # s) h \<leadsto>\<^sub>s StackState (Eval (Var x)) s h" 
 | ret_tyapp [simp]: 
     "StackState (Return (VTyAbs k e)) (STyApp t # s) h \<leadsto>\<^sub>s StackState (Eval (subst\<^sub>t\<^sub>e 0 t e)) s h" 
 
@@ -51,6 +51,10 @@ lemma vcanonical_forall [simp]: "\<Delta>,\<Gamma> \<turnstile>\<^sub>v v : Fora
   by (induction \<Gamma> v "Forall k t" rule: typecheck_value.induct) auto
 
 lemma lookup_in_tc [simp]: "\<Delta>,\<Gamma> \<turnstile>\<^sub>x\<^sub>s xs : ts \<Longrightarrow> lookup l ts = Some t \<Longrightarrow> \<exists>x. lookup l xs = Some x"
+  by (induction l xs arbitrary: ts rule: lookup.induct) auto
+
+lemma lookup_in_env [simp]: "\<Delta>,\<Gamma> \<turnstile>\<^sub>x\<^sub>s xs : ts \<Longrightarrow> lookup l ts = Some t \<Longrightarrow> lookup l xs = Some x \<Longrightarrow> 
+    lookup x \<Gamma> = Some t"
   by (induction l xs arbitrary: ts rule: lookup.induct) auto
 
 lemma "\<Delta>,\<Gamma> \<turnstile> e : t \<Longrightarrow> True"
@@ -126,36 +130,66 @@ theorem preservation: "\<Sigma> \<leadsto>\<^sub>s \<Sigma>' \<Longrightarrow> \
   next case (ev_app e\<^sub>1 e\<^sub>2 s h)
     then obtain \<Gamma> t\<^sub>1 t\<^sub>2 where "(\<Gamma> \<turnstile>\<^sub>s\<^sub>s s : t\<^sub>2 \<rightarrow> t) \<and> ([],\<Gamma> \<turnstile> e\<^sub>1 : Arrow t\<^sub>1 t\<^sub>2) \<and> 
       ([],\<Gamma> \<turnstile> e\<^sub>2 : t\<^sub>1) \<and> (h \<turnstile>\<^sub>h \<Gamma>)" by blast
-    moreover hence "\<Gamma> \<turnstile>\<^sub>s\<^sub>s SApp e\<^sub>2 # s : Arrow t\<^sub>1 t\<^sub>2 \<rightarrow> t" by (metis tc_sapp tcs_cons)
-    ultimately show ?case by simp
+    thus ?case by (metis tc_sapp tcs_cons tc_eval_state)
   next case (ev_let e\<^sub>1 e\<^sub>2 s h)
     then obtain \<Gamma> t\<^sub>1 t\<^sub>2 where T: "(\<Gamma> \<turnstile>\<^sub>s\<^sub>s s : t\<^sub>2 \<rightarrow> t) \<and> ([],\<Gamma> \<turnstile> e\<^sub>1 : t\<^sub>1) \<and> 
       ([],insert_at 0 t\<^sub>1 \<Gamma> \<turnstile> e\<^sub>2 : t\<^sub>2) \<and> (h \<turnstile>\<^sub>h \<Gamma>)" by blast
-    hence L: "length\<^sub>h h = length \<Gamma>" by blast
-    from T have X: "insert_at (length \<Gamma>) t\<^sub>1 \<Gamma> \<turnstile>\<^sub>s\<^sub>s s : t\<^sub>2 \<rightarrow> t" by simp
+    hence X: "insert_at (length\<^sub>h h) t\<^sub>1 \<Gamma> \<turnstile>\<^sub>s\<^sub>s s : t\<^sub>2 \<rightarrow> t" by fastforce 
     from T have "[],insert_at (length (insert_at 0 t\<^sub>1 \<Gamma>)) t\<^sub>1 (insert_at 0 t\<^sub>1 \<Gamma>) \<turnstile> e\<^sub>2 : t\<^sub>2" 
-      using tc_weaken by blast
-    with L have Y: "[],insert_at 0 t\<^sub>1 (insert_at (length\<^sub>h h) t\<^sub>1 \<Gamma>) \<turnstile> e\<^sub>2 : t\<^sub>2" by simp
-    from L have "lookup (length\<^sub>h h) (insert_at (length\<^sub>h h) t\<^sub>1 \<Gamma>) = Some t\<^sub>1" by simp
-    with T X Y show ?case by simp
-  next case ev_proj 
-    thus ?case by metis
-  next case ev_case 
-    thus ?case by metis
-  next case ev_unfold 
-    thus ?case by metis
-  next case ev_tyapp 
-    thus ?case by metis
-  next case ret_ref 
-    thus ?case by metis
-  next case ret_app 
-    thus ?case by metis
-  next case ret_proj 
-    thus ?case by metis
-  next case ret_case 
-    thus ?case by metis
-  next case ret_tyapp 
-    thus ?case by metis
+      by (metis tc_weaken)
+    hence "[],insert_at 0 t\<^sub>1 (insert_at (length \<Gamma>) t\<^sub>1 \<Gamma>) \<turnstile> e\<^sub>2 : t\<^sub>2" by simp
+    moreover from T have "length\<^sub>h h = length \<Gamma>" by blast
+    ultimately have "[],insert_at (length\<^sub>h h) t\<^sub>1 \<Gamma> \<turnstile> subst\<^sub>x\<^sub>e 0 (length\<^sub>h h) e\<^sub>2 : t\<^sub>2" by simp
+    with T X show ?case by simp
+  next case (ev_proj e l s h)
+    then obtain \<Gamma> tt ts where "(\<Gamma> \<turnstile>\<^sub>s\<^sub>s s : tt \<rightarrow> t) \<and> ([],\<Gamma> \<turnstile> e : Record ts) \<and> 
+      lookup l ts = Some tt \<and> (h \<turnstile>\<^sub>h \<Gamma>)" by blast
+    thus ?case by (metis tc_sproj tcs_cons tc_eval_state)
+  next case (ev_case e t' cs s h)
+    then obtain \<Gamma> ts where "(\<Gamma> \<turnstile>\<^sub>s\<^sub>s s : t' \<rightarrow> t) \<and> ([],\<Gamma> \<turnstile> e : Variant ts) \<and> 
+      ([],\<Gamma> \<turnstile>\<^sub>c cs : ts \<rightarrow> t') \<and> (h \<turnstile>\<^sub>h \<Gamma>)" by blast
+    thus ?case by (metis tc_scase tcs_cons tc_eval_state)
+  next case (ev_unfold tt e s h)
+    then obtain \<Gamma> k where T: "(\<Gamma> \<turnstile>\<^sub>s\<^sub>s s : subst\<^sub>t\<^sub>t 0 (Inductive k tt) tt \<rightarrow> t) \<and> 
+      ([],\<Gamma> \<turnstile> e : Inductive k tt) \<and> (insert_at 0 k [] \<turnstile>\<^sub>k tt : Star) \<and> (h \<turnstile>\<^sub>h \<Gamma>)" by blast
+    moreover hence "[k] \<turnstile>\<^sub>k tt : Star" by simp
+    ultimately show ?case by (metis tc_eval_state tcs_cons tc_sunfold)
+  next case (ev_tyapp e tt s h)
+    then obtain \<Gamma> k t' where "(\<Gamma> \<turnstile>\<^sub>s\<^sub>s s : subst\<^sub>t\<^sub>t 0 tt t' \<rightarrow> t) \<and> ([],\<Gamma> \<turnstile> e : Forall k t') \<and> 
+      ([] \<turnstile>\<^sub>k tt : k) \<and> (h \<turnstile>\<^sub>h \<Gamma>)" by blast
+    thus ?case by (metis tc_eval_state tcs_cons tc_styapp)
+  next case (ret_ref v x s h)
+    then obtain \<Gamma> t' where "lookup x \<Gamma> = Some t' \<and> (\<Gamma> \<turnstile>\<^sub>s\<^sub>s s : t' \<rightarrow> t) \<and> ([],\<Gamma> \<turnstile>\<^sub>v v : t') \<and> 
+      (h \<turnstile>\<^sub>h \<Gamma>)" by blast
+    moreover hence "update\<^sub>h h x (devalue v) \<turnstile>\<^sub>h \<Gamma>" by simp
+    ultimately show ?case by (metis tc_return_state)
+  next case (ret_app t\<^sub>1 e\<^sub>1 e\<^sub>2 s h)
+    then obtain \<Gamma> t\<^sub>2 where T: "([],\<Gamma> \<turnstile> e\<^sub>2 : t\<^sub>1) \<and> (\<Gamma> \<turnstile>\<^sub>s\<^sub>s s : t\<^sub>2 \<rightarrow> t) \<and> 
+      ([],insert_at 0 t\<^sub>1 \<Gamma> \<turnstile> e\<^sub>1 : t\<^sub>2) \<and> ([] \<turnstile>\<^sub>k t\<^sub>1 : Star) \<and> (h \<turnstile>\<^sub>h \<Gamma>)" by blast
+    hence X: "insert_at (length\<^sub>h h) t\<^sub>1 \<Gamma> \<turnstile>\<^sub>s\<^sub>s s : t\<^sub>2 \<rightarrow> t" by fastforce
+    from T have "length\<^sub>h h = length \<Gamma>" by blast
+    moreover from T have "[],insert_at (length (insert_at 0 t\<^sub>1 \<Gamma>)) t\<^sub>1 (insert_at 0 t\<^sub>1 \<Gamma>) \<turnstile> e\<^sub>1 : t\<^sub>2" 
+      by (metis tc_weaken)
+    ultimately have "[],insert_at (length\<^sub>h h) t\<^sub>1 \<Gamma> \<turnstile> subst\<^sub>x\<^sub>e 0 (length\<^sub>h h) e\<^sub>1 : t\<^sub>2" by simp
+    with T X show ?case by fastforce
+  next case (ret_proj l xs x s h)
+    moreover then obtain \<Gamma> ts t' where "(lookup l ts = Some t') \<and> (\<Gamma> \<turnstile>\<^sub>s\<^sub>s s : t' \<rightarrow> t) \<and> 
+      ([],\<Gamma> \<turnstile>\<^sub>x\<^sub>s xs : ts) \<and> (h \<turnstile>\<^sub>h \<Gamma>)" by blast
+    ultimately show ?case by (metis tc_eval_state tc_var lookup_in_env)
+  next case (ret_case l cs e ts x tt s h) 
+    then obtain \<Gamma> t' where T: "([],\<Gamma> \<turnstile>\<^sub>c cs : ts \<rightarrow> tt) \<and> (\<Gamma> \<turnstile>\<^sub>s\<^sub>s s : tt \<rightarrow> t) \<and> 
+      lookup x \<Gamma> = Some t' \<and> lookup l ts = Some t' \<and> (\<forall>tt \<in> set ts. [] \<turnstile>\<^sub>k tt : Star) \<and> (h \<turnstile>\<^sub>h \<Gamma>)" 
+        by blast
+    moreover with ret_case have "[],insert_at 0 t' \<Gamma> \<turnstile> e : tt" by auto
+    ultimately have "[],\<Gamma> \<turnstile> subst\<^sub>x\<^sub>e 0 x e : tt" by simp
+    with T show ?case by (metis tc_eval_state)
+  next case (ret_tyapp k e tt s h)
+    then obtain \<Gamma> t' where T: "([] \<turnstile>\<^sub>k tt : k) \<and> (\<Gamma> \<turnstile>\<^sub>s\<^sub>s s : subst\<^sub>t\<^sub>t 0 tt t' \<rightarrow> t) \<and> 
+      (insert_at 0 k [],map (incr\<^sub>t\<^sub>t 0) \<Gamma> \<turnstile> e : t') \<and> (h \<turnstile>\<^sub>h \<Gamma>)" by blast
+    hence "[],map (subst\<^sub>t\<^sub>t 0 tt) (map (incr\<^sub>t\<^sub>t 0) \<Gamma>) \<turnstile> subst\<^sub>t\<^sub>e 0 tt e : subst\<^sub>t\<^sub>t 0 tt t'" 
+      using tc_subst\<^sub>t\<^sub>e by blast
+    hence "[],\<Gamma> \<turnstile> subst\<^sub>t\<^sub>e 0 tt e : subst\<^sub>t\<^sub>t 0 tt t'" by simp
+    with T show ?case by (metis tc_eval_state)
   qed fastforce+
 
 end
