Index.thy
@@ -1,0 +1,19 @@
+theory Index
+imports Vector
+begin
+
+definition incr :: "nat \<Rightarrow> nat \<Rightarrow> nat" where
+  "incr x y = (if x \<le> y then Suc y else y)"
+
+definition decr :: "nat \<Rightarrow> nat \<Rightarrow> nat" where
+  "decr x y = (if x < y then y - 1 else y)"
+
+lemma [simp]: "lookup y as = Some a \<Longrightarrow> x \<le> length as \<Longrightarrow> 
+    lookup (incr x y) (insert_at x a' as) = Some a"
+  by (simp add: incr_def)
+
+lemma [simp]: "lookup y (insert_at x a' as) = Some a \<Longrightarrow> x \<le> length as \<Longrightarrow> 
+    lookup x' as = Some a' \<Longrightarrow> x \<noteq> y \<Longrightarrow> lookup (decr x y) as = Some a"
+  by (cases y) (auto simp add: decr_def)
+
+end
